minor proof changes

Fair.v
@@ -30,65 +30,64 @@ Hint Resolve same_ask_is_fair same_bid_is_fair.
 
 (*------------ Sorting by decreasing bid prices and their properties --------------*)
 
-Definition b_by_bp (b1:Bid) (b2:Bid) := (b2 <=? b1).
+Definition by_bp (b1:Bid) (b2:Bid) := (b2 <=? b1).
 
-Lemma b_by_bp_P : transitive b_by_bp /\ comparable b_by_bp.
+Lemma by_bp_P : transitive by_bp /\ comparable by_bp.
 Proof.  { split.
-          
-          { unfold transitive. unfold b_by_bp.  
+          { unfold transitive. unfold by_bp.  
             intros y x z H H1. move /leP in H1. move /leP in H.
             apply /leP. omega. }
-          { unfold comparable.  unfold b_by_bp. intros.
+          { unfold comparable.  unfold by_bp. intros.
            move /leP in H. apply /leP. omega. } } Qed.
             
  
-Definition a_by_sp (a1:Ask) (a2:Ask) := a1 <=? a2.
+Definition m_bp (m1:fill_type) (m2:fill_type) := by_bp (bid_of m1) (bid_of m2).
 
-Lemma a_by_sp_P : transitive a_by_sp /\ comparable a_by_sp.
+Lemma m_bp_P : transitive m_bp /\ comparable m_bp.
 Proof. { split.
-         { unfold transitive. unfold a_by_sp.  
+         { unfold transitive. unfold m_bp. 
+           intros. cut (transitive by_bp). intros. eauto using by_bp_P. 
+            apply by_bp_P. }
+         { unfold comparable.  unfold m_bp. intros x y H. eapply by_bp_P. 
+           exact.  } } Qed.
+
+(*------------- Sorting by increasing ask prices and their properties -------------*)
+
+Definition by_sp (a1:Ask) (a2:Ask) := a1 <=? a2.
+
+Lemma by_sp_P : transitive by_sp /\ comparable by_sp.
+Proof. { split.
+         { unfold transitive. unfold by_sp.  
             intros y x z H H1. move /leP in H1. move /leP in H.
             apply /leP. omega. }
-          { unfold comparable.  unfold a_by_sp. intros.
+          { unfold comparable.  unfold by_sp. intros.
            move /leP in H. apply /leP. omega. } } Qed.
 
+Definition m_sp (m1:fill_type) (m2:fill_type) :=  by_sp (ask_of m1) (ask_of m2).
 
-Definition m_by_bp (m1:fill_type) (m2:fill_type) := 
-b_by_bp (bid_of m1) (bid_of m2).
-Lemma m_by_bp_P : transitive m_by_bp /\ comparable m_by_bp.
+Lemma m_sp_P : transitive m_sp /\ comparable m_sp.
 Proof. { split.
-         { unfold transitive. unfold m_by_bp. 
-           intros. cut (transitive b_by_bp). intros. eauto using b_by_bp_P. 
-            apply b_by_bp_P. }
-         { unfold comparable.  unfold m_by_bp. intros x y H. eapply b_by_bp_P. 
+         { unfold transitive. unfold m_sp. 
+           intros. cut (transitive by_sp). intros. eauto using by_sp_P. 
+            apply by_sp_P. }
+         { unfold comparable.  unfold m_sp. intros x y H. eapply by_sp_P. 
            exact.  } } Qed. 
 
-Definition m_by_sp (m1:fill_type) (m2:fill_type) := 
- a_by_sp (ask_of m1) (ask_of m2).
-Lemma m_by_sp_P : transitive m_by_sp /\ comparable m_by_sp.
-Proof. { split.
-         { unfold transitive. unfold m_by_sp. 
-           intros. cut (transitive a_by_sp). intros. eauto using a_by_sp_P. 
-            apply a_by_sp_P. }
-         { unfold comparable.  unfold m_by_sp. intros x y H. eapply a_by_sp_P. 
-           exact.  } } Qed. 
-
-Hint Resolve m_by_bp_P m_by_sp_P b_by_bp_P a_by_sp_P.
+Hint Resolve m_bp_P m_sp_P by_bp_P by_sp_P.
 
  
 Lemma top_prices_mb (m: fill_type)(b: Bid) (M: list fill_type)(B: list Bid):
-  Sorted m_by_bp (m::M)-> Sorted b_by_bp (b::B) -> 
-  bids_of (m::M) [<=] (b::B) -> (bid_of m) <= b.
+  Sorted m_bp (m::M)-> Sorted by_bp (b::B) ->  bids_of (m::M) [<=] (b::B) -> (bid_of m) <= b.
 Proof. Admitted.
 
 
 Lemma tail_is_matching (m: fill_type)(b: Bid) (M: list fill_type)(B: list Bid)(A: list Ask):
-  Sorted m_by_bp (m::M)-> Sorted b_by_bp (b::B) -> matching_in (b::B) A (m::M)->
-  matching_in B A M.
+  Sorted m_bp (m::M)-> Sorted by_bp (b::B) -> matching_in (b::B) A (m::M)-> matching_in B A M.
 Proof. Admitted.
 
   
 (*----------------  Function to make a matching fair on bids -----------------*)
+
 Fixpoint Make_FOB (M:list fill_type) (B: list Bid):=
 match (M,B) with 
 |(nil,_) => nil
@@ -97,18 +96,16 @@ match (M,B) with
 end.
 
 
-Lemma mfob_subB (M:list fill_type) (B:list Bid) :
-bids_of (Make_FOB M B) [<=] B.
-Proof. { revert B. induction M. simpl. auto.
-intro B. case B. simpl. auto. intros b l. simpl.
-intro x. intro H1. destruct H1. subst x. auto.
-cut (In x l). auto. eapply IHM. exact. } Qed.  
+Lemma mfob_subB (M:list fill_type) (B:list Bid): bids_of (Make_FOB M B) [<=] B.
+Proof. { revert B. induction M. simpl. auto. intro B.
+         case B.
+         { simpl. auto. }
+         { intros b l. simpl. intro x. intro H1.
+           destruct H1. subst x. auto. cut (In x l). auto. eapply IHM. auto. } } Qed.  
 
-
-Lemma mfob_matchable (M:list fill_type) (B:list Bid) (NDB: NoDup B):
-(Sorted m_by_bp M) -> (Sorted b_by_bp B) -> All_matchable M
--> bids_of M [<=] B -> NoDup (bids_of M) -> All_matchable (Make_FOB M B).
-
+Lemma mfob_matchable (M:list fill_type)(B:list Bid)(NDB: NoDup B):
+  (Sorted m_bp M) -> (Sorted by_bp B) -> All_matchable M -> bids_of M [<=] B ->
+   NoDup (bids_of M) -> All_matchable (Make_FOB M B).
 Proof. revert B NDB. induction M. 
        { intros B H1 H2 H3 H4 H5 H6. simpl. eauto. }
        { intros B H1 H2 H3 H4 H5 H6. 
@@ -117,16 +114,22 @@ Proof. revert B NDB. induction M.
           { simpl. apply All_matchable_intro. 
           { simpl.
             assert (H7: b >= (bid_of a)). 
-            { eapply top_prices_mb. eauto. eauto. exact. } 
+            { eapply top_prices_mb. eauto. eauto. auto. } 
             assert (H8: bid_of a >= ask_of a). 
-            { unfold All_matchable in H4. simpl in H4. eapply H4. left. auto. }
-            omega. }
+            { unfold All_matchable in H4. simpl in H4. eapply H4. left;auto. }
+            omega. } 
           { eapply IHM. 
             { eauto. } 
             { eauto. }
             { eauto. } 
             { eapply All_matchable_elim1. eauto. }
-            { admit. }
+            { (*--- bids_of M [<=] B ----*)
+              intros x H7.
+              assert (H8: In x (b::B)).
+              { apply H5. simpl. right;auto. }
+              assert (H9: x <> b).
+              { 
+              eauto.  }
             { simpl in H6. eauto. } Admitted.   
         
 
@@ -140,20 +143,16 @@ Proof.
 *)
 
 Lemma mfob_matching (M:list fill_type) (B:list Bid) (A:list Ask) (NDB: NoDup B):
-(Sorted m_by_bp M) -> (Sorted b_by_bp B) -> (matching_in B A M) -> matching (Make_FOB M B).
-
+(Sorted m_bp M) -> (Sorted by_bp B) -> (matching_in B A M) -> matching (Make_FOB M B).
 Proof. Admitted.
  
 
-
 Lemma mfob_subA (M:list fill_type) (B:list Bid) (A:list Ask):
-(Sorted m_by_bp M) -> (Sorted b_by_bp B) -> (matching_in B A M) -> 
-(asks_of (Make_FOB M B)) [<=] A.
+(Sorted m_bp M) -> (Sorted by_bp B) -> (matching_in B A M) -> (asks_of (Make_FOB M B)) [<=] A.
  Proof. Admitted.
 
 Lemma mfob_matching_in (M: list fill_type)(B: list Bid)(A: list Ask)(NDB: NoDup B):
-(Sorted m_by_bp M) -> (Sorted b_by_bp B) -> matching_in B A M ->
-matching_in B A (Make_FOB M B) .
+(Sorted m_bp M) -> (Sorted by_bp B) -> matching_in B A M -> matching_in B A (Make_FOB M B) .
 Proof.  { intros H1 H2 H3. unfold matching_in. 
           split. { eapply mfob_matching. all: auto. eapply H3.  }
                  split. { eapply mfob_subB. }
@@ -161,46 +160,41 @@ Proof.  { intros H1 H2 H3. unfold matching_in.
 
 
 
-
-
 Lemma mfob_asks_is_perm (M: list fill_type) (B:list Bid):
 perm (asks_of M) (asks_of (Make_FOB M B)). 
 Proof. Admitted. 
-
 
 Lemma mfob_is_same_size (M: list fill_type) (B:list Bid):
 |M| = |(Make_FOB M B)|. 
 Proof. Admitted.
 
-
 Lemma mfob_fair_on_bid (M: list fill_type) (B:list Bid) (A:list Ask):
- (Sorted m_by_bp M) -> (Sorted b_by_bp B) -> matching_in B A M ->
- fair_on_bids (Make_FOB M B) B. 
+ (Sorted m_bp M) -> (Sorted by_bp B) -> matching_in B A M -> fair_on_bids (Make_FOB M B) B. 
 Proof. Admitted.  
 
 Hint Resolve mfob_matching mfob_asks_is_perm mfob_is_same_size mfob_fair_on_bid.
 
-Theorem exists_fair_on_bids (M: list fill_type) (B: list Bid) (A:list Ask)(NDB: NoDup B):
+Theorem exists_fair_on_bids (M: list fill_type) (B: list Bid)(A:list Ask)(NDB: NoDup B):
   matching_in B A M->
   (exists M':list fill_type, matching_in B A M'  /\ (|M| = |M'|) /\ perm (asks_of M) (asks_of M')
    /\ fair_on_bids M' B).
-Proof.  { assert (HmP: transitive m_by_bp /\ comparable m_by_bp). apply m_by_bp_P.  
-        assert (HbP: transitive b_by_bp /\ comparable b_by_bp). apply b_by_bp_P.
+Proof. { assert (HmP: transitive m_bp /\ comparable m_bp). apply m_bp_P.  
+        assert (HbP: transitive by_bp /\ comparable by_bp). apply by_bp_P.
         destruct HmP as [Hmp1 Hmp2]. destruct HbP as [Hbp1 Hbp2].
-        intro H. exists (Make_FOB (sort m_by_bp M) (sort b_by_bp B)).
+        intro H. exists (Make_FOB (sort m_bp M) (sort by_bp B)).
         split. 
-        { assert (HM: matching_in (sort b_by_bp B) A (Make_FOB (sort m_by_bp M) (sort b_by_bp B))).
+        { assert (HM: matching_in (sort by_bp B) A (Make_FOB (sort m_bp M) (sort by_bp B))).
           apply mfob_matching_in. all:auto. 
           apply match_inv with (M:=M)(B:=B)(A:=A);auto.
           eapply match_inv with
-              (B:= (sort b_by_bp B)) (M:=(Make_FOB (sort m_by_bp M) (sort b_by_bp B))) (A:=A).
+              (B:= (sort by_bp B)) (M:=(Make_FOB (sort m_bp M) (sort by_bp B))) (A:=A).
           all: auto. } split.
-        { replace (|M|) with (|sort m_by_bp M|); auto. } split.
-        {  assert(HA: perm (asks_of (sort m_by_bp M))
-                          (asks_of (Make_FOB (sort m_by_bp M) (sort b_by_bp B)))).
+        { replace (|M|) with (|sort m_bp M|); auto. } split.
+        {  assert(HA: perm (asks_of (sort m_bp M))
+                          (asks_of (Make_FOB (sort m_bp M) (sort by_bp B)))).
           auto. eauto with auction.  }
         {  assert (HBid: fair_on_bids
-                           (Make_FOB (sort m_by_bp M) (sort b_by_bp B)) (sort b_by_bp B)).
+                           (Make_FOB (sort m_bp M) (sort by_bp B)) (sort by_bp B)).
            eapply mfob_fair_on_bid. all:auto. eapply match_inv with (M:=M)(B:=B)(A:=A);auto.
            eauto with auction. } } Qed.
 
@@ -230,6 +224,6 @@ Proof. { intros H0. apply exists_fair_on_bids in H0 as H1.
        { auto. }
        split.
        { split. auto. eauto. }
-       {eauto. } exact. } Qed.
+       {eauto. } auto. } Qed.
          
 End Fair.
